src/Blocking.v
@@ -30,46 +30,13 @@ Definition Blocked (msgs: MessagePool TMsg) :=
     tinfo_rqin ti1 = tinfo_rqin ti2 ->
     ti1 = ti2.
 
+(** An informal high-level goal statement:
+ * Certain shape of [Rule]s ->
+ * [BlockedInv] ->
+ * [ValidTrss] /\ [SimMP]
+ *)
 Definition BlockedInv (tst: TState) :=
   Blocked (tst_msgs tst).
-
-(* This statement looks a bit weird at first glance, since the "first-to-first"
- * property is applied for all internal messages for which [FirstMP] holds.
- * However, it's true since [Blocked] guarantees that given a certain channel 
- * only a single set of messages (originated from the channel) are in
- * [MessagePool]. And those messages are the oldest ones for each channel,
- * which are mapped to the "first" message in spec.
- *)
-Theorem blocked_int_SimMP_FirstMP:
-  forall ist,
-    Blocked ist ->
-    forall (impl: System) sst,
-      SimMP msgP impl ist sst ->
-      forall imsg,
-        toInternal impl imsg = true ->
-        FirstMP ist imsg ->
-        forall smsg,
-          smsg = deinitialize msgP imsg ->
-          FirstMP sst smsg.
-Proof.
-Admitted.
-
-Corollary blocked_SimMP_FirstMP_map:
-  forall ist,
-    Blocked ist ->
-    forall (impl: System) msgP sst,
-      SimMP msgP impl ist sst ->
-      forall imsgs,
-        Forall (fun msg => toInternal impl msg = true) imsgs ->
-        Forall (FirstMP ist) imsgs ->
-        forall smsgs,
-          smsgs = deinitializeMP msgP imsgs ->
-          Forall (FirstMP sst) smsgs.
-Proof.
-  induction imsgs; intros; subst; [constructor|].
-  inv H1; inv H2; constructor; eauto.
-  eapply blocked_int_SimMP_FirstMP; eauto.
-Qed.
 
 Lemma BlockedInv_MsgsInv:
   MsgsInv BlockedInv.
@@ -78,22 +45,22 @@ Proof.
   - hnf; intros.
     hnf; hnf in H; intros.
     cbn in *.
-    apply in_app_or in H0; destruct H0.
-    + apply in_app_or in H1; destruct H1.
-      * eauto.
-      * exfalso; clear -H1 H3.
-        induction eins; simpl; auto.
-        inv H1; auto.
-        discriminate.
+    apply InMP_enqMsgs_or in H0; destruct H0.
     + exfalso; clear -H0 H2.
       induction eins; simpl; auto.
       inv H0; auto.
-      discriminate.
+      inv H; discriminate.
+    + apply InMP_enqMsgs_or in H1; destruct H1.
+      * exfalso; clear -H1 H3.
+        induction eins; simpl; auto.
+        inv H1; auto.
+        inv H; discriminate.
+      * eauto.
   - hnf; intros.
     hnf; hnf in H; intros.
     cbn in *.
-    apply InMP_removeMsgs in H0.
-    apply InMP_removeMsgs in H1.
+    apply InMP_deqMsgs in H0.
+    apply InMP_deqMsgs in H1.
     eauto.
 Qed.
 
