src/Reduction.v
@@ -10,99 +10,6 @@ Ltac dest_step_m :=
          | [H: {| bst_oss := _ |} = {| bst_oss := _ |} |- _] => inv H
          end; simpl in *.
 
-Definition EquivMState (st1 st2: MState) :=
-  bst_oss st1 = bst_oss st2 /\
-  bst_orqs st1 = bst_orqs st2 /\
-  EquivMP (bst_msgs st1) (bst_msgs st2).
-
-Ltac dest_equivM :=
-  repeat
-    match goal with
-    | [H: EquivMState _ _ |- _] => red in H; dest; simpl in *; subst
-    | [H: ?t = ?t |- _] => clear H
-    end.
-
-Ltac split_equivM :=
-  split; [|split]; simpl.
-
-Lemma EquivMState_refl:
-  forall st, EquivMState st st.
-Proof.
-  intros; split_equivM; auto.
-  apply EquivMP_refl.
-Qed.
-
-Lemma EquivMState_sym:
-  forall st1 st2, EquivMState st1 st2 -> EquivMState st2 st1.
-Proof.
-  intros; dest_equivM; split_equivM; auto.
-  apply EquivMP_sym; auto.
-Qed.
-
-Lemma EquivMState_trans:
-  forall st1 st2 st3,
-    EquivMState st1 st2 ->
-    EquivMState st2 st3 ->
-    EquivMState st1 st3.
-Proof.
-  intros; dest_equivM; split_equivM.
-  - rewrite H; auto.
-  - rewrite H3; auto.
-  - eapply EquivMP_trans; eauto.
-Qed.
-
-Lemma EquivMState_step_m:
-  forall sys st1 lbl st2,
-    step_m sys st1 lbl st2 ->
-    forall cst1,
-      EquivMState st1 cst1 ->
-      exists cst2,
-        step_m sys cst1 lbl cst2 /\ EquivMState st2 cst2.
-Proof.
-  intros.
-  inv H.
-  - exists cst1; split; auto.
-    constructor.
-  - destruct cst1 as [coss1 corqs1 cmsgs1].
-    dest_equivM; eexists; split.
-    + econstructor; eauto.
-    + split_equivM; auto.
-      apply EquivMP_distributeMsgs; auto.
-  - destruct cst1 as [coss1 corqs1 cmsgs1].
-    dest_equivM; eexists; split.
-    + eapply SmOuts; try reflexivity; eauto.
-      eapply EquivMP_Forall_FirstMP; eauto.
-    + split_equivM; auto.
-      apply EquivMP_removeMsgs; auto.
-  - destruct cst1 as [coss1 corqs1 cmsgs1].
-    dest_equivM; eexists; split.
-    + econstructor; try reflexivity; try eassumption.
-      eapply EquivMP_Forall_FirstMP; eauto.
-    + split_equivM; auto.
-      apply EquivMP_distributeMsgs.
-      apply EquivMP_removeMsgs.
-      auto.
-Qed.
-
-Lemma EquivMState_steps_t:
-  forall sys st1 hst st2,
-    steps step_m sys st1 hst st2 ->
-    forall cst1,
-      EquivMState st1 cst1 ->
-      exists cst2,
-        steps step_m sys cst1 hst cst2 /\ EquivMState st2 cst2.
-Proof.
-  induction 1; simpl; intros.
-  - exists cst1; split; auto.
-    constructor.
-  - specialize (IHsteps _ H1); destruct IHsteps as [csti [? ?]].
-    eapply EquivMState_step_m in H0; eauto.
-    destruct H0 as [cst2 [? ?]].
-    eexists; split.
-    + econstructor; eassumption.
-    + assumption.
-Qed.
-
 Definition NonSilentHistory (hst: History) :=
   Forall (fun lbl => lbl <> emptyRLabel _) hst.
 
@@ -119,149 +26,63 @@ Lemma msg_ins_commutes:
   forall sys st1 eins lbl st2,
     NotMsgIn lbl ->
     steps step_m sys st1 [RlblIns eins; lbl] st2 ->
-    forall cst1,
-      EquivMState st1 cst1 ->
-      exists cst2,
-        steps step_m sys cst1 [lbl; RlblIns eins] cst2 /\
-        EquivMState st2 cst2.
+    steps step_m sys st1 [lbl; RlblIns eins] st2.
 Proof.
   intros.
   destruct lbl as [|hdl mins mouts|]; [elim H| |].
-  - destruct cst1 as [coss1 corqs1 cmsgs1].
-    dest_step_m.
-    + eexists; split.
+  - dest_step_m.
+    + econstructor.
       * econstructor.
-        { econstructor.
-          { econstructor. }
-          { econstructor; eauto. }
-        }
         { econstructor. }
-      * dest_equivM.
-        repeat split.
-        apply EquivMP_distributeMsgs; auto.
-    + dest_equivM.
-      eexists; split.
+        { econstructor; eauto. }
       * econstructor.
-        { econstructor.
-          { econstructor. }
-          { econstructor; eauto. }
-        }
-        { econstructor; try reflexivity; try eassumption.
-          clear -H4 H10; eapply Forall_impl.
-          { clear; intros; simpl in H.
-            apply FirstMP_distributeMsgs; eassumption.
-          }
-          { eapply Forall_impl; [|eassumption].
-            intros.
-            eapply EquivMP_FirstMP; eauto.
-          }
-        }
-      * repeat split; simpl.
-        rewrite FirstMP_removeMsgs_distributeMsgs_comm.
-        { unfold enqMP, distributeMsgs.
-          do 2 rewrite <-app_assoc.
-          apply EquivMP_app.
-          { apply EquivMP_removeMsgs; auto. }
-          { assert (NoDup (map msgAddrOf mouts)).
-            { eapply ValidMsgsOut_MsgAddr_NoDup in H17; eauto. }
-            assert (NoDup ((map msgAddrOf eins))).
-            { destruct H3; assumption. }
-            pose proof (ValidMsgsOut_ValidMsgsExtIn_DisjList H5 H17 H3).
-
-            apply EquivMP_MsgAddr_NoDup_EquivList.
-            { rewrite map_app; apply NoDup_DisjList; auto. }
-            { rewrite map_app; apply NoDup_DisjList; auto.
-              apply DisjList_comm; auto.
-            }
-            { apply EquivList_app_comm. }
-          }
-        }
-        { eapply ValidMsgsIn_MsgAddr_NoDup; eauto. }
-        { eapply EquivMP_Forall_FirstMP; eauto. }
-  - destruct cst1 as [coss1 corqs1 cmsgs1].
-    dest_step_m.
-    dest_equivM.
-    eexists; split.
     + econstructor.
       * econstructor.
         { econstructor. }
         { econstructor; eauto. }
       * econstructor; try reflexivity; try eassumption.
-        clear -H3 H7; eapply Forall_impl; [|eassumption].
-        intros; apply FirstMP_distributeMsgs.
-        eapply EquivMP_FirstMP; eauto.
-    + repeat split; simpl.
-      rewrite FirstMP_removeMsgs_distributeMsgs_comm.
-      { apply EquivMP_distributeMsgs.
-        apply EquivMP_removeMsgs.
-        assumption.
-      }
-      { destruct H4; assumption. }
-      { eapply EquivMP_Forall_FirstMP; eauto. }
-Qed.
+        { admit. }
+        { f_equal.
+          admit.
+        }
+  - dest_step_m.
+    econstructor.
+    + econstructor.
+      * econstructor.
+      * econstructor; eauto.
+    + econstructor; try reflexivity; try eassumption.
+      * admit.
+      * f_equal.
+        admit.
+Admitted.
 
 Lemma msg_in_reduced:
   forall sys st1 eins hst2 st2,
     steps step_m sys st1 (RlblIns eins :: hst2) st2 ->
     NonMsgInHistory hst2 ->
-    forall cst1,
-      EquivMState st1 cst1 ->
-      exists cst2,
-        steps step_m sys cst1 (hst2 ++ [RlblIns eins]) cst2 /\
-        EquivMState st2 cst2.
+    steps step_m sys st1 (hst2 ++ [RlblIns eins]) st2.
 Proof.
-  induction hst2 as [|lbl ?]; simpl; intros.
-  - dest_step_m.
-    destruct cst1 as [coss1 corqs1 cmsgs1].
-    exists {| bst_oss := coss1; bst_orqs := corqs1;
-              bst_msgs := distributeMsgs eins cmsgs1 |}; split.
-    + econstructor.
-      * econstructor.
-      * econstructor; eauto.
-    + dest_equivM; split_equivM; auto.
-      apply EquivMP_distributeMsgs; auto.
-      
-  - inv H0.
-    change (RlblIns eins :: lbl :: hst2) with ([RlblIns eins; lbl] ++ hst2) in H.
-    eapply steps_split in H; [|reflexivity].
-    destruct H as [sti [? ?]].
-    eapply msg_ins_commutes in H0; [|assumption|apply EquivMState_refl].
-    destruct H0 as [cst2 [? ?]].
-    pose proof (steps_append H H0); inv H3.
-    specialize (IHhst2 _ H9 H5 _ H1).
-    destruct IHhst2 as [icst2 [? ?]].
-    eapply EquivMState_step_m in H11; [|eassumption].
-    destruct H11 as [cst3 [? ?]].
-    exists cst3; split.
-    + econstructor; eauto.
-    + eapply EquivMState_trans; eauto.
+  induction hst2 as [|lbl ?]; simpl; intros; auto.
+  inv H0.
+  change (RlblIns eins :: lbl :: hst2) with ([RlblIns eins; lbl] ++ hst2) in H.
+  eapply steps_split in H; [|reflexivity].
+  destruct H as [sti [? ?]].
+  eapply msg_ins_commutes in H0; [|assumption].
+  pose proof (steps_append H H0); inv H1.
+  specialize (IHhst2 _ H7 H4).
+  econstructor; eauto.
 Qed.
 
 Lemma msg_in_reduced_app:
   forall sys st1 hst1 eins hst2 st2,
     steps step_m sys st1 (hst1 ++ RlblIns eins :: hst2) st2 ->
     NonMsgInHistory hst2 ->
-    forall cst1,
-      EquivMState st1 cst1 ->
-      exists cst2,
-        steps step_m sys cst1 (hst1 ++ hst2 ++ [RlblIns eins]) cst2 /\
-        EquivMState st2 cst2.
+    steps step_m sys st1 (hst1 ++ hst2 ++ [RlblIns eins]) st2.
 Proof.
   intros.
   eapply steps_split in H; [|reflexivity].
   destruct H as [sti [? ?]].
   eapply msg_in_reduced in H; eauto.
-  destruct H as [csti [? ?]].
-  eapply EquivMState_steps_t in H2; eauto.
-  destruct H2 as [cst2 [? ?]].
-  exists cst2; split.
-  - eapply steps_append; eauto.
-  - assumption.
+  eapply steps_append; eauto.
 Qed.
-
-Definition NonInterfering (rule1 rule2: Rule)
-           (mins1 mins2 mouts1 mouts2: list Msg) :=
-  rule_oidx rule1 <> rule_oidx rule2 /\
-  DisjList (map msgAddrOf mins1) (map msgAddrOf mins2) /\
-  DisjList (map msgAddrOf mouts1) (map msgAddrOf mins2).
 
