src/StepPred.v
@@ -8,28 +8,14 @@ Section GivenMsg.
   Variable (MsgT StateT LabelT: Type).
   Context `{HasMsg MsgT} `{HasLabel LabelT}.
 
-  Definition ResponsesOk (origRq: PMsg MsgT)
-             (rss: list (PMsg MsgT)) (opred: OPred) (rsbf: RsBackF) :=
-    forall poss noss post nost,
-      Forall (fun rs =>
-                (pred_os (pmsg_pred rs) (pmsg_val origRq) poss (pmsg_val rs) noss))
-             rss ->
-      poss@[mid_to (pmsg_mid origRq)] = Some post ->
-      noss@[mid_to (pmsg_mid origRq)] = Some nost ->
-      opred (pmsg_val origRq) post
-            (rsbf (map (fun pmsg => msg_value (getMsg pmsg)) rss) nost) nost ->
-      (pred_os (pmsg_pred origRq) (pmsg_val origRq) poss
-               (rsbf (map (fun pmsg => msg_value (getMsg pmsg)) rss) nost)) noss.
-
-  Definition toOrigMP (mp: MessagePool (PMsg MsgT)): MessagePool MsgT :=
-    map (@pmsg_omsg _) mp.
+  Definition toOrigMP {MsgT} := mpmap (@pmsg_omsg MsgT).
 
   Inductive step_pred0 (psys: PSystem MsgT):
     PState MsgT -> PLabel MsgT -> PState MsgT -> Prop :=
   | SpSlt: forall st, step_pred0 psys st (emptyPLabel MsgT) st
 
   | SpIns:
-      forall pst nst oss oims orqs (eins: list (PMsg MsgT)),
+      forall pst nst oss oims orqs (eins: list (Id (PMsg MsgT))),
         eins <> nil ->
         ValidMsgsExtIn psys eins ->
         pst = {| pst_oss := oss;
@@ -37,11 +23,11 @@ Section GivenMsg.
                  pst_msgs := oims |} ->
         nst = {| pst_oss := oss;
                  pst_orqs := orqs;
-                 pst_msgs := distributeMsgs eins oims |} ->
+                 pst_msgs := enqMsgs eins oims |} ->
         step_pred0 psys pst (PlblIns eins) nst
 
   | SpOuts:
-      forall pst nst oss oims orqs (eouts: list (PMsg MsgT)),
+      forall pst nst oss oims orqs (eouts: list (Id (PMsg MsgT))),
         eouts <> nil ->
         ValidMsgsExtOut psys eouts ->
         pst = {| pst_oss := oss;
@@ -49,27 +35,27 @@ Section GivenMsg.
                  pst_msgs := oims |} ->
         nst = {| pst_oss := oss;
                  pst_orqs := orqs;
-                 pst_msgs := removeMsgs eouts oims |} ->
+                 pst_msgs := deqMsgs (idsOf eouts) oims |} ->
         step_pred0 psys pst (PlblOuts eouts) nst
 
   | SpImm:
       forall pst nst poss noss oidx pos nos orqs porq poims noims
-             (immr: PRule MsgT) prec (rq: PMsg MsgT) (rs: PMsg MsgT),
-        In oidx (indicesOf psys) ->
+             (immr: PRule MsgT) prec (rq: Id (PMsg MsgT)) (rs: Id (PMsg MsgT)),
+        In oidx (oindsOf psys) ->
         In immr (psys_rules psys) ->
-        immr = PRuleImm (pmsg_pmid rq) (pmsg_pmid rs) prec ->
-        DualPMsg rq rs ->
-        FirstMP poims rq ->
-        ValidMsgsIn oidx (rq :: nil) ->
+        immr = PRuleImm oidx (pmidOf rq) (pmidOf rs) prec ->
+        (* DualPMsg rq rs -> *)
+        FirstMPI poims rq ->
+        ValidMsgsIn psys (rq :: nil) ->
 
         poss@[oidx] = Some pos ->
         orqs@[oidx] = Some porq ->
-        prec pos (map (fun pmsg => getMsg (pmsg_omsg pmsg)) porq) (getMsg rq :: nil) ->
-        pred_os (pmsg_pred rq) (pmsg_val rq) poss (pmsg_val rs) noss ->
-        pred_mp (pmsg_pred rq) (toOrigMP poims) (toOrigMP noims) ->
+        prec pos (map (fun pmsg => getMsg (pmsg_omsg pmsg)) porq) (liftI getMsg rq :: nil) ->
+        pred_os (pmsg_pred (valOf rq)) (pmsg_val (valOf rq)) poss (pmsg_val (valOf rs)) noss ->
+        pred_mp (pmsg_pred (valOf rq)) (toOrigMP poims) (toOrigMP noims) ->
 
         noss = poss +[ oidx <- nos ] ->
-        noims = distributeMsgs (intOuts psys (rs :: nil)) (removeMP rq poims) ->
+        noims = enqMPI rq (deqMP (idOf rq) poims) ->
 
         pst = {| pst_oss := poss; pst_orqs := orqs; pst_msgs := poims |} ->
         nst = {| pst_oss := noss; pst_orqs := orqs; pst_msgs := noims |} ->
@@ -79,64 +65,60 @@ Section GivenMsg.
   | SpRqFwd:
       forall pst nst oss porq orqs oidx pos oims
              (rqfwdr: PRule MsgT) prec
-             (rq: PMsg MsgT) (fwds: list (PMsg MsgT)),
-        In oidx (indicesOf psys) ->
+             (rq: Id (PMsg MsgT)) (fwds: list (Id (PMsg MsgT))),
+        In oidx (oindsOf psys) ->
         In rqfwdr (psys_rules psys) ->
-        rqfwdr = PRuleRqFwd (pmsg_pmid rq) prec (map (@pmsg_pmid _ _) fwds) ->
-        FirstMP oims rq ->
-        ValidMsgsIn oidx (rq :: nil) ->
-        ValidMsgsOut oidx fwds ->
+        rqfwdr = PRuleRqFwd oidx (pmidOf rq) prec (map (@pmidOf _ _) fwds) ->
+        FirstMPI oims rq ->
+        ValidMsgsIn psys (rq :: nil) ->
+        ValidMsgsOut fwds ->
 
         oss@[oidx] = Some pos ->
-        prec pos (map (fun pmsg => getMsg (pmsg_omsg pmsg)) porq) (getMsg rq :: nil) ->
+        prec pos (map (fun pmsg => getMsg (pmsg_omsg pmsg)) porq) (liftI getMsg rq :: nil) ->
 
         orqs@[oidx] = Some porq ->
 
         pst = {| pst_oss := oss; pst_orqs := orqs; pst_msgs := oims |} ->
         nst = {| pst_oss := oss;
-                 pst_orqs := orqs +[ oidx <- addRq porq rq ];
-                 pst_msgs := distributeMsgs
-                               (intOuts psys fwds)
-                               (removeMP rq oims) |} ->
+                 pst_orqs := orqs +[ oidx <- addRq porq (valOf rq) ];
+                 pst_msgs := enqMsgs fwds (deqMP (idOf rq) oims) |} ->
 
         step_pred0 psys pst (PlblInt (Some rqfwdr) (rq :: nil) fwds) nst
 
   | SpRsBack:
       forall pst nst oss orqs oidx pos nos orq origRq oims noss noims opred rsbf
-             (rsbackr: PRule MsgT) (rss: list (PMsg MsgT)) (rsb: PMsg MsgT),
-        In oidx (indicesOf psys) ->
+             (rsbackr: PRule MsgT) (rss: list (Id (PMsg MsgT))) (rsb: Id (PMsg MsgT)),
+        In oidx (oindsOf psys) ->
         In rsbackr (psys_rules psys) ->
-        rsbackr = PRuleRsBack (map (@pmsg_pmid _ _) rss) opred
-                              (pmsg_pmid rsb) rsbf  ->
-        Forall (FirstMP oims) rss ->
-        ValidMsgsIn oidx rss ->
-        ValidMsgsOut oidx (rsb :: nil) ->
+        rsbackr = PRuleRsBack oidx (map (@pmidOf _ _) rss) opred (pmidOf rsb) rsbf  ->
+        Forall (FirstMPI oims) rss ->
+        ValidMsgsIn psys rss ->
+        ValidMsgsOut (rsb :: nil) ->
 
         oss@[oidx] = Some pos ->
         orqs@[oidx] = Some orq ->
-        getRq (fun pmsg => mid_tid (pmid_mid (pmsg_pmid pmsg)))
-              orq (mid_tid (pmid_mid (pmsg_pmid rsb))) = Some origRq ->
+        getRq (fun pmsg => msg_id (getMsg (pmsg_omsg pmsg)))
+              orq (msg_id (getMsg (pmsg_omsg (valOf rsb)))) = Some origRq ->
 
         noss = oss +[ oidx <- nos ] ->
-        noims = distributeMsgs
-                  (intOuts psys (rsb :: nil))
-                  (removeMsgs rss oims) ->
+        noims = enqMsgs (rsb :: nil) (deqMsgs (idsOf rss) oims) ->
         
         (* Backing responses are all valid. *)
         Forall (fun pmsg =>
                   pred_os (pmsg_pred pmsg) (msg_value (getMsg (pmsg_omsg origRq))) oss
                           (pmsg_val pmsg) (oss +[ oidx <- nos ]) /\
                   pred_mp (pmsg_pred pmsg) (toOrigMP oims)
-                          (toOrigMP (enqMP rsb (removeMsgs rss oims)))) rss ->
-        opred (msg_value (getMsg (pmsg_omsg origRq))) pos (pmsg_val rsb) nos ->
-        pmsg_val rsb = rsbf (map (fun pmsg => msg_value (getMsg pmsg)) rss) pos ->
+                          (toOrigMP (enqMPI rsb (deqMsgs (idsOf rss) oims))))
+               (valsOf rss) ->
+        opred (msg_value (getMsg (pmsg_omsg origRq))) pos (pmsg_val (valOf rsb)) nos ->
+        pmsg_val (valOf rsb) = rsbf (map (fun idp => msg_value (getMsg (valOf idp))) rss) pos ->
 
         (* Using such responses, we should be able to prove 
          * the original request predicate.
          *)
-        pred_os (pmsg_pred rsb) (msg_value (getMsg (pmsg_omsg origRq)))
-                oss (pmsg_val rsb) noss ->
-        pred_mp (pmsg_pred rsb) (toOrigMP oims) (toOrigMP noims) ->
+        pred_os (pmsg_pred (valOf rsb)) (msg_value (getMsg (pmsg_omsg origRq)))
+                oss (pmsg_val (valOf rsb)) noss ->
+        pred_mp (pmsg_pred (valOf rsb)) (toOrigMP oims) (toOrigMP noims) ->
 
         pst = {| pst_oss := oss;
                  pst_orqs := orqs;
